Makefile
@@ -78,7 +78,7 @@ endif
 .PHONY: 3d-exe
 
 # lowparse needed because of .fst behind .fsti for extraction
-3d-pulse-prelude: $(filter-out src/lowparse/LowParse.SLow.% src/lowparse/LowParse.Low.%,$(filter src/lowparse/%,$(ALL_CHECKED_FILES))) $(filter lib/everparse/3d/%,$(ALL_CHECKED_FILES))
+3d-pulse-prelude: $(filter-out $(LOWPARSE_LOW_FILTER),$(filter src/lowparse/%,$(ALL_CHECKED_FILES))) $(filter lib/everparse/3d/%,$(ALL_CHECKED_FILES))
 
 .PHONY: 3d-pulse-prelude
 
